Use a generic cx

src/statics.lean
@@ -1,28 +1,17 @@
 import syntax
 
-inductive cx: Type
-| nil: cx
-| cons: cx -> var -> typ -> cx
+inductive val_typ: cx typ -> val -> typ -> Prop
+| int (Γ: cx typ) (n: ℤ): val_typ Γ (val.int n) typ.int
+| true (Γ: cx typ): val_typ Γ val.true typ.bool
+| false (Γ: cx typ): val_typ Γ val.false typ.bool
 
-inductive lookup: cx -> var -> typ -> Prop
-| hd (Γ: cx) (x: var) (τ: typ): lookup (cx.cons Γ x τ) x τ
-| tl (Γ: cx) (x: var) (y: var) (τ: typ) (τ': typ):
-    x ≠ y ->
-    lookup Γ x τ ->
-    lookup (cx.cons Γ y τ') x τ
-
-inductive val_typ: cx -> val -> typ -> Prop
-| int (Γ: cx) (n: ℤ): val_typ Γ (val.int n) typ.int
-| true (Γ: cx): val_typ Γ val.true typ.bool
-| false (Γ: cx): val_typ Γ val.false typ.bool
-
-inductive exp_typ: cx -> exp -> typ -> Prop
+inductive exp_typ: cx typ -> exp -> typ -> Prop
 | pure
-    (Γ: cx) (v: val) (τ: typ):
+    (Γ: cx typ) (v: val) (τ: typ):
     val_typ Γ v τ ->
     exp_typ Γ (exp.pure v) τ
 | if_
-    (Γ: cx)
+    (Γ: cx typ)
     (e1: exp) (e2: exp) (e3: exp) (τ: typ):
     exp_typ Γ e1 typ.bool ->
     exp_typ Γ e2 τ ->
