src/dynamics.lean
@@ -1,20 +1,16 @@
 import syntax
 
-inductive vcx: Type
-| nil: vcx
-| cons: vcx -> var -> val -> vcx
-
-inductive steps: vcx -> exp -> exp -> Prop
+inductive steps: cx val -> exp -> exp -> Prop
 | if_e1
-    (Δ: vcx)
+    (Δ: cx val)
     (e1: exp) (e1': exp) (e2: exp) (e3: exp):
     steps Δ e1 e1' ->
     steps Δ (exp.if_ e1 e2 e3) (exp.if_ e1' e2 e3)
 | if_true
-    (Δ: vcx)
+    (Δ: cx val)
     (e2: exp) (e3: exp):
     steps Δ (exp.if_ (exp.pure val.true) e2 e3) e2
 | if_false
-    (Δ: vcx)
+    (Δ: cx val)
     (e2: exp) (e3: exp):
     steps Δ (exp.if_ (exp.pure val.false) e2 e3) e3
