src/safety.lean
@@ -1,11 +1,9 @@
 import helpers
 
--- seems like we have to write this as taking in a general context and also a
--- proof that it is nil, rather than just having `et: has_typ cx.nil e tau`.
 theorem progress
-  (Γ: cx) (Δ: vcx)
-  (cx_nil: Γ = cx.nil)
-  (vcx_nil: Δ = vcx.nil)
+  (Γ: cx typ) (Δ: cx val)
+  (tcx_nil: Γ = cx.nil typ)
+  (vcx_nil: Δ = cx.nil val)
   (e: exp) (τ: typ)
   (et: exp_typ Γ e τ)
   : (∃ (v: val), e = exp.pure v) ∨ (∃ (e': exp), steps Δ e e') :=
@@ -15,7 +13,7 @@ begin
   existsi et_v,
   refl,
   right,
-  cases et_ih_a cx_nil,
+  cases et_ih_a tcx_nil,
   cases h,
   rewrite h_h at *,
   cases bool_canonical_forms et_Γ h_w (inversion_pure et_Γ h_w typ.bool et_a),
@@ -31,9 +29,9 @@ begin
 end
 
 theorem preservation
-  (Γ: cx) (Δ: vcx)
-  (cx_nil: Γ = cx.nil)
-  (vcx_nil: Δ = vcx.nil)
+  (Γ: cx typ) (Δ: cx val)
+  (tcx_nil: Γ = cx.nil typ)
+  (vcx_nil: Δ = cx.nil val)
   (e: exp) (e': exp) (τ: typ)
   (et: exp_typ Γ e τ)
   (st: steps Δ e e')
@@ -41,7 +39,7 @@ theorem preservation
 begin
   induction st generalizing Γ τ,
   let inv := inversion_if Γ st_e1 st_e2 st_e3 τ et,
-  let e1_typ := st_ih vcx_nil Γ typ.bool cx_nil inv.left,
+  let e1_typ := st_ih vcx_nil Γ typ.bool tcx_nil inv.left,
   exact exp_typ.if_ Γ st_e1' st_e2 st_e3 τ e1_typ inv.right.left inv.right.right,
   let inv := inversion_if Γ (exp.pure val.true) st_e2 st_e3 τ et,
   exact inv.right.left,
