src/var.lean
@@ -1,0 +1,13 @@
+-- any infinite set would work
+def var: Type := string
+
+inductive cx (t: Type): Type
+| nil: cx
+| cons: cx -> var -> t -> cx
+
+inductive lookup (t: Type): cx t -> var -> t -> Prop
+| hd (Γ: cx t) (x: var) (out: t): lookup (cx.cons Γ x out) x out
+| tl (Γ: cx t) (x: var) (out: t) (y: var) (out_y: t):
+    x ≠ y ->
+    lookup Γ x out ->
+    lookup (cx.cons Γ y out_y) x out
